theories/HOU/std/lists/misc.v
@@ -6,12 +6,12 @@ Lemma list_decompose k {X} (A: list X):
   k <= length A -> exists A1 A2, A = A1 ++ A2 /\ length A1 = k.
 Proof.
   induction A in k |-*; intros.
-  - exists nil. exists nil; cbn. destruct k; intuition.
+  - exists nil. exists nil; cbn. destruct k; intuition easy.
   - destruct k.
-    + exists nil; exists (a :: A); intuition.
+    + exists nil; exists (a :: A); intuition easy.
     + cbn in *; assert (k <= length A) by lia. destruct (IHA _ H0) as (A1 & A2 & ?).
-      intuition. exists (a :: A1). exists A2. subst. 
-      intuition.
+      intuition idtac. exists (a :: A1). exists A2. subst. 
+      intuition easy.
 Qed.
 
 Lemma list_decompose_alt k {X} (A: list X):
@@ -20,34 +20,9 @@ Proof.
   intros H.
   assert (length A - k <= length A) by lia.
   destruct (list_decompose _ H0) as (A1 & A2 & ?).
-  intuition. exists A1. exists A2. intuition.
+  intuition idtac. exists A1. exists A2. intuition idtac.
   specialize (app_length A1 A2) as H4.
   rewrite <-H2 in H4. rewrite H4 in H3. lia.
-Qed.
-
-
-Lemma list_decompose_end {X} (A: list X):
-  A = nil \/ exists a' A', A = A' ++ [a'].
-Proof.
-  induction A; intuition; subst.
-  all: right; try destruct IH as (a' & A' & ?).
-  + exists a. exists nil. reflexivity.
-  + destruct H as (a' & A' & ?); subst.
-    exists a'. exists (a :: A'). reflexivity.
-Qed.
-
-
-
-Lemma list_decompose_strong Y k (A: list Y):
-  k <= length A -> { A1 & { A2 | A = A1 ++ A2 /\ length A1 = k}}.
-Proof.
-  induction A in k |-*; intros H.
-  - exists nil. exists nil. intuition.
-  - destruct k.
-    + exists nil. exists (a :: A). intuition.
-    + cbn in H; eapply le_S_n in H.
-      destruct (IHA _ H) as (A1 & A2 & H1 & H2); subst.
-      exists (a :: A1). exists A2. intuition.
 Qed.
 
 Lemma list_pointwise_eq X (A B: list X):
@@ -62,24 +37,13 @@ Proof.
     intros x; exact (H (S x)).
 Qed.
 
-Lemma list_end_ind:
-  forall (A : Type) (P : list A -> Prop),
-    P [] ->
-    (forall (a : A) (l : list A), P l -> P (l ++ [a])) -> forall l : list A, P l.
-Proof.
-  intros A P H IH l.
-  specialize (rev_list_ind P H) as Ind.
-  rewrite <-rev_involutive. eapply Ind.
-  intros; cbn; now apply IH.
-Qed.
-
 Lemma app_injective {X} (A B C D: list X):
   length A = length C -> A ++ B = C ++ D -> A = C /\ B = D.
 Proof.
   induction A in C |-*; destruct C; try discriminate.
-  cbn; intuition.
+  cbn; intuition easy.
   injection 1 as ?. injection 1 as ?.
-  subst. edestruct IHA; eauto; subst; intuition.
+  subst. edestruct IHA; eauto; subst; intuition easy.
 Qed.
 
 Lemma app_injective_right Y (A1 A2 B1 B2 : list Y):
@@ -87,5 +51,5 @@ Lemma app_injective_right Y (A1 A2 B1 B2 : list Y):
 Proof.
   intros H; induction A1 in B1 |-*; destruct B1; cbn; eauto.
   1 - 2: intros; subst; cbn in H; autorewrite with list in H; lia.  
-  intros [= -> ? % IHA1]; intuition; now subst.
+  intros [= -> ? % IHA1]; intuition idtac; now subst.
 Qed.
