theories/HOU/unification/unification.v
@@ -1,3 +1,2 @@
 From Undecidability.HOU.unification Require Export
-    higher_order_unification systemunification nth_order_unification
-    enumerability.
+    higher_order_unification systemunification nth_order_unification.
