theories/StackMachines/Util/Nat_facts.v
@@ -1,4 +1,4 @@
-Require Import Arith Lia.
+Require Import Arith Lia ZArith.Znat ZArith.Zdiv.
 
 Require Import ssreflect ssrbool ssrfun.
 
@@ -6,18 +6,41 @@ Set Default Goal Selector "!".
 
 Definition nat_norm := (Nat.add_0_r, Nat.add_succ_r, Nat.sub_0_r, Nat.mul_1_r, Nat.div_1_r).
 
+Lemma div_exact (a b : nat) : a = b * (a / b) <-> a mod b = 0.
+Proof.
+  rewrite [X in X = _](Nat.div_mod_eq a b). lia.
+Qed.
+
+Lemma add_mod (a b n : nat) : (a + b) mod n = (a mod n + b mod n) mod n.
+Proof.
+  apply: Nat2Z.inj. do ? rewrite !(Nat2Z.inj_mod, Nat2Z.inj_add).
+  apply: Zplus_mod.
+Qed.
+
+Lemma mod_same (a : nat) : a mod a = 0.
+Proof.
+  apply: Nat2Z.inj. rewrite Nat2Z.inj_mod.
+  apply: Z_mod_same_full.
+Qed.
+
+Lemma mod_mod (a n : nat) : (a mod n) mod n = a mod n.
+Proof.
+  apply: Nat2Z.inj. rewrite !Nat2Z.inj_mod.
+  apply: Zmod_mod.
+Qed.
+
 Lemma div_mod_pos {n m: nat} : S m / (1 + n) + S m mod (1 + n) <> 0.
 Proof.
-  move=> ?. 
+  move=> ?.
   have /Nat.div_small_iff : S m / (1 + n) = 0 by lia. move /(_ ltac:(lia)).
-  have /Nat.div_exact : S m mod (1 + n) = 0 by lia. move /(_ ltac:(lia)).
+  have /div_exact : S m mod (1 + n) = 0 by lia.
   by lia.
 Qed.
 
 Lemma divides_frac_diff {m n} : m mod (n + 1) = 0 -> (m * (n + 2) / (n + 1) - m) * (1 + n) = m.
 Proof.
   rewrite Nat.mul_sub_distr_r.
-  move=> /Nat.div_exact => /(_ ltac:(lia)) ?.
+  move=> /div_exact => ?.
   have -> : m * (n + 2) = ((n+2) * (m / (n + 1))) * (n + 1) by lia.
   by rewrite Nat.div_mul; lia.
 Qed.
